continue working on LayoutIR

theories/compiler/layout.v
@@ -1,10 +1,17 @@
 From Coq Require Import List NArith.BinNat Lists.List.
-From stdpp Require Import base option strings list pretty.
+From stdpp Require Import base option strings list pretty decidable.
 From Wasm Require datatypes.
 From RWasm Require term annotated_term.
 From RWasm.compiler Require Import numbers monads.
 
 Section Layout.
+  Inductive LayoutPrimType :=
+  | LT_int
+  | LT_float.
+
+  Inductive LayoutPrimSize :=
+  | LS32
+  | LS64.
 
   Inductive LayoutShape :=
   | LS_int32
@@ -19,6 +26,63 @@ Section Layout.
   | LV_float32 (f : nat)
   | LV_float64 (f : nat)
   | LV_tuple (fields : list LayoutValue).
+
+  Global Instance layout_prim_type_eq_dec : EqDecision LayoutPrimType.
+  Proof. solve_decision. Defined.
+
+  Global Instance layout_prim_size_eq_dec : EqDecision LayoutPrimSize.
+  Proof. solve_decision. Defined.
+
+  Fixpoint layout_shape_eq_dec (x y : LayoutShape) : {x = y} + {x ≠ y}.
+  Proof. decide equality; solve_decision. Defined.
+
+  Global Instance layout_shape_eq_dec_inst : EqDecision LayoutShape := layout_shape_eq_dec.
+
+  Fixpoint layout_value_eq_dec (x y : LayoutValue) : {x = y} + {x ≠ y}.
+  Proof. decide equality; solve_decision. Defined.
+
+  Global Instance layout_value_eq_dec_inst : EqDecision LayoutValue := layout_value_eq_dec.
+
+  Global Instance pretty_layout_shape : Pretty LayoutShape :=
+    fix go (sh : LayoutShape) : string :=
+      match sh with
+      | LS_int32 => "i32"
+      | LS_int64 => "i64"
+      | LS_float32 => "f32"
+      | LS_float64 => "f64"
+      | LS_tuple fields =>
+          String.app (String.app "(" (String.concat ", " (map go fields))) ")"
+      end.
+
+  Definition layout_prim_size (ls : LayoutShape) : option LayoutPrimSize :=
+    match ls with
+    | LS_int32 => Some LS32
+    | LS_int64 => Some LS64
+    | LS_float32 => Some LS32
+    | LS_float64 => Some LS64
+    | LS_tuple _ => None
+    end.
+
+  Definition layout_size_of_int (int : term.IntType) : LayoutPrimSize :=
+    match int with
+    | term.i32 => LS32
+    | term.i64 => LS64
+    end.
+  Definition layout_size_of_float (float : term.FloatType) : LayoutPrimSize :=
+    match float with
+    | term.f32 => LS32
+    | term.f64 => LS64
+    end.
+  Definition layout_int_from_sz (sz : LayoutPrimSize) : LayoutShape :=
+    match sz with
+    | LS32 => LS_int32
+    | LS64 => LS_int64
+    end .
+  Definition layout_float_from_sz (sz : LayoutPrimSize) : LayoutShape :=
+    match sz with
+    | LS32 => LS_float32
+    | LS64 => LS_float64
+    end.
 
   Fixpoint layout_value_to_shape (lv : LayoutValue) : LayoutShape :=
     match lv with
