theories/compiler/ir.v
@@ -1,9 +1,8 @@
 From Coq Require Import List NArith.BinNat Lists.List.
-From stdpp Require Import base option strings list pretty.
+From stdpp Require Import base option strings list pretty decidable gmap.
 From Wasm Require datatypes.
 From RWasm Require term annotated_term.
 From RWasm.compiler Require Import numbers monads.
-
 
 Module BoxPolymorphicIR.
 
@@ -61,7 +60,7 @@ Module BoxPolymorphicIR.
   | Drop
   | Select
   | Block (tf : ArrowType) (le : LocalEffect) (e__s : list Instruction)
-  | Loop (tf : ArrowType) (e : list Instruction)
+  | Loop (tf : ArrowType) (e__s : list Instruction)
   | ITE (tf : ArrowType) (le : LocalEffect) (e__thn : list Instruction) (e__els : list Instruction)
   | Br (i : nat)
   | Br_if (i : nat)
@@ -204,10 +203,10 @@ Module BoxPolymorphicIR.
     | AR.Free => mthrow (err "unexpected admin instr")
     end.
 End BoxPolymorphicIR.
+
 Module LayoutIR.
 
-  From RWasm.compiler Require Import layout.
-
+  From RWasm.compiler Require Export layout.
   Definition shape := LayoutShape.
   Definition value := LayoutValue.
 
@@ -249,6 +248,282 @@ Module LayoutIR.
   | Free
 
   | VariantCase (q : rwasm.Qual) (ψ : rwasm.HeapType) (tf : ArrowShape) (le : LocalEffect) (e__ss : list (list Instruction)) (* FIXME *)
-  .
-  
-End Layout.
+  with Func :=
+  | Fun (ex__s : list rwasm.ex) (tf : ArrowShape) (e__s : list Instruction).
+
+  Inductive Glob :=
+  | GlobMut (shape : shape) (i__s : list Instruction)
+  | GlobEx (ex__s : list rwasm.ex) (shape : shape) (i__s : list Instruction)
+  | GlobIm (ex__s : list rwasm.ex) (shape : shape) (im : rwasm.im).
+
+  Record module := {
+    functions : list Func;
+    globals : list Glob;
+    table : rwasm.Table
+  }.
+
+  Record TypeEnv := {
+    te_locals  : gmap nat shape;
+    te_globals : gmap nat (bool * shape);
+    (* TODO: this might need to keep track of tables too *)
+    te_stack   : list shape
+  }.
+
+  Definition te_push (s : LayoutShape) (Γ : TypeEnv) : TypeEnv :=
+    {| te_locals := Γ.(te_locals);
+       te_globals := Γ.(te_globals);
+       te_stack := s :: Γ.(te_stack) |}.
+
+  Definition te_pop (Γ : TypeEnv) : option (LayoutShape * TypeEnv) :=
+    match Γ.(te_stack) with
+    | [] => None
+    | s :: stk' =>
+      Some (s, {| te_locals := Γ.(te_locals);
+                  te_globals := Γ.(te_globals);
+                  te_stack := stk' |})
+    end.
+
+
+  Definition either_layout_num (sz : LayoutPrimSize) (lt : LayoutPrimType) :=
+    match lt with
+    | LT_int => layout_int_from_sz sz
+    | LT_float => layout_float_from_sz sz
+    end.
+
+  Definition either_single (sz : LayoutPrimSize) (l : list LayoutPrimType) :=
+    map (either_layout_num sz) l.
+
+  Definition either_n (sz : LayoutPrimSize) (ls : (list LayoutPrimType) * (list LayoutPrimType))
+        : (list LayoutShape) * (list LayoutShape) :=
+    let '(l1, l2) := ls in
+    ((map (either_layout_num sz) l1), (map (either_layout_num sz) l2)).
+
+  Definition rwasm_i_to_layout_prim (i : rwasm.IntType) :=
+    match i with
+    | rwasm.i32 => LS_int32
+    | rwasm.i64 => LS_int64
+    end.
+  Definition rwasm_f_to_layout_prim (f : rwasm.FloatType) :=
+    match f with
+    | rwasm.f32 => LS_float32
+    | rwasm.f64 => LS_float64
+    end.
+
+  Definition apply_tf (tf : ArrowShape) (Γ : TypeEnv) : M TypeEnv :=
+    let 'Arrow shapes__in shapes__out := tf in
+    Γ1 ← foldlM (fun (shape : LayoutShape) (acc : TypeEnv) =>
+          '(shape', acc') ← lift_optionM (te_pop acc) "expected non-empty stack when applying arrow shape";
+          match decide (shape = shape') with
+          | left _ => mret acc'
+          | right _ => mthrow (err ("Based on arrow shape, expected " ++ (pretty shape) ++ " but got " ++ (pretty shape') ++ " at TOS."))
+          end) Γ shapes__in;
+    Γ2 ← mret $ foldl' te_push Γ1 shapes__out;
+    mret Γ2.
+
+  Fixpoint type_instr (instr : Instruction) (Γ : TypeEnv) : M TypeEnv :=
+    match instr with
+    | Const v => mret $ te_push (layout_value_to_shape v) Γ
+    | Ne ni =>
+      let szi := layout_size_of_int in
+      let szf := layout_size_of_float in
+      let lsi := rwasm_i_to_layout_prim in
+      let lsf := rwasm_f_to_layout_prim in
+      let '(tin, tout) := match ni with
+      | rwasm.Iu i _ => either_n (szi i) ([LT_int], [LT_int])
+      | rwasm.Ib i _ => either_n (szi i) ([LT_int; LT_int], [LT_int])
+      | rwasm.Fu f _ => either_n (szf f) ([LT_float], [LT_float])
+      | rwasm.Fb f _ => either_n (szf f) ([LT_float; LT_float], [LT_float])
+      | rwasm.It i _ => either_n (szi i) ([LT_int], [LT_int])
+      | rwasm.Ir i _ => (either_single (szi i) [LT_int; LT_int], [LS_int32])
+      | rwasm.Fr f _ => (either_single (szf f) [LT_float; LT_float], [LS_int32])
+      | rwasm.CvtI i1 op =>
+        match op with
+        | rwasm.Wrap i2 => ([lsi i2], [lsi i1])
+        | rwasm.Extend i2 _ => ([lsi i2], [lsi i1])
+        | rwasm.Trunc f2 _ => ([lsf f2], [lsi i1])
+        | rwasm.TruncSat f2 _ =>([lsf f2], [lsi i1])
+        | rwasm.Convert i2 _ => ([lsi i2], [lsi i1])
+        | rwasm.Demote f2 => ([lsf f2], [lsi i1])
+        | rwasm.Promote f2 => ([lsf f2], [lsi i1])
+        | rwasm.Reinterpret i2 => ([lsi i2], [lsi i1])
+        (* FIXME: missing reinterpret for floats *)
+        end
+      | rwasm.CvtF f1 op =>
+        match op with
+        | rwasm.Wrap i2 => ([lsi i2], [lsf f1])
+        | rwasm.Extend i2 _ => ([lsi i2], [lsf f1])
+        | rwasm.Trunc f2 _ => ([lsf f2], [lsf f1])
+        | rwasm.TruncSat f2 _ =>([lsf f2], [lsf f1])
+        | rwasm.Convert i2 _ => ([lsi i2], [lsf f1])
+        | rwasm.Demote f2 => ([lsf f2], [lsf f1])
+        | rwasm.Promote f2 => ([lsf f2], [lsf f1])
+        | rwasm.Reinterpret i2 => ([lsi i2], [lsf f1])
+        end
+      end in
+
+      Γ1 ← foldlM (fun (shape : LayoutShape) (acc : TypeEnv) =>
+             '(shape', acc') ← lift_optionM (te_pop acc) "expected non-empty stack";
+             match decide (shape = shape') with
+             | left _ => mret acc'
+             | right _ => mthrow (err ("Expected " ++ (pretty shape) ++ " but got " ++ (pretty shape') ++ " at TOS."))
+             end) Γ tin;
+      Γ2 ← mret $ foldl' te_push Γ1 tout;
+      mret Γ2
+    | Unreachable => mret Γ
+    | Nop => mret Γ
+    | Drop =>
+      '(shape, Γ') ← lift_optionM (te_pop Γ) "Drop: expected non-empty stack";
+      mret Γ'
+    | Select =>
+      '(shape1, Γ1) ← lift_optionM (te_pop Γ) "Select: expected non-empty stack 1";
+      '(shape2, Γ2) ← lift_optionM (te_pop Γ1) "Select: expected non-empty stack 2";
+      '(shape3, Γ3) ← lift_optionM (te_pop Γ2) "Select: expected non-empty stack 3";
+      _ ← match shape1 with
+      | LS_int32 => mret ()
+      | _ => mthrow (err ("Select expected i32 at TOS but got " ++ (pretty shape1)))
+      end;
+      Γ4 ← match decide (shape2 = shape3) with
+      | left _ => mret (te_push shape2 Γ3)
+      | right _ => mthrow (err ("Expected equal shapes for select but got " ++ (pretty shape2) ++ " and " ++ (pretty shape3) ++ "."))
+      end;
+      mret Γ3
+    | Block tf le e__s =>
+      (* TODO: validate that tf and le are correct? *)
+      Γ__arrow ← apply_tf tf Γ;
+      Γ__locals ← apply_le le Γ__arrow;
+      mret Γ__locals
+    | Loop tf e__s =>
+      (* TODO: validate that tf is correct? *)
+      Γ' ← apply_tf tf Γ;
+      mret Γ'
+    | ITE tf le e__thn e__els =>
+      (* TODO: validate that tf and le are correct? *)
+      Γ__arrow ← apply_tf tf Γ;
+      Γ__locals ← apply_le le Γ__arrow;
+      mret Γ__locals
+    | Br i
+    | Br_if i
+    | Br_table i__s j => mthrow (err "TODO: deal with labels")
+    | Ret => mthrow (err "TODO:")
+    (* | GetLocal i => _ *)
+    (* | SetLocal i => _ *)
+    (* | TeeLocal i => _ *)
+    (* | GetGlobal i => _ *)
+    (* | SetGlobal i => _ *)
+    (* | CallIndirect tf => _ *)
+    (* | Call i => _ *)
+    (* | LoadOffset offset => _ *)
+    (* | StoreOffset offset => _ *)
+    (* | SwapOffset offset => _ *)
+    (* | Malloc shape => _ *)
+    (* | Free => _ *)
+    | VariantCase q ψ tf le e__ss => mthrow (err "NEEDED?")
+    | _ => mthrow (err "TODO")   (*  *)
+   end.
+
+
+End LayoutIR.
+
+Section AddIfNotIn.
+  Context `{EqDecision A}.
+
+  Fixpoint add_if_not_in (x : A) (l : list A) : list A :=
+    if bool_decide (x ∈ l) then l else x :: l.
+End AddIfNotIn.
+
+Module LayoutToWasm.
+  Import LayoutIR.
+  From RWasm.compiler Require Import numbers monads.
+
+  Definition translate_function_type (tf : ArrowShape) : wasm.function_type :=
+    match tf with
+    | Arrow s1 s2 =>
+       let s1' := flat_map shape_to_wasm_types s1 in
+       let s2' := flat_map shape_to_wasm_types s2 in
+       wasm.Tf s1' s2'
+    end.
+
+  Section Instrs.
+
+    Variable function_types : list wasm.function_type.
+
+    Fixpoint compile_val (value : LayoutValue) : list wasm.value :=
+      match value with
+      | LV_int32 i => [compile_num_from_Z wasm.T_i32 (Z.of_nat i)]
+      | LV_int64 i => [compile_num_from_Z wasm.T_i64 (Z.of_nat i)]
+      | LV_float32 f => [compile_num_from_Z wasm.T_f32 (Z.of_nat f)]
+      | LV_float64 f => [compile_num_from_Z wasm.T_f64 (Z.of_nat f)]
+      | LV_tuple fields => flat_map compile_val fields
+      end.
+
+    Definition compile_instr (instr : Instruction) (Γ : TypeEnv) : InstM (list wasm.basic_instruction) :=
+      match instr with
+      | Const v =>
+          let wasm_vals := compile_val v in
+          mret $ map wasm.BI_const wasm_vals
+      | Ne ni =>
+          instr ← liftM (compile_num_intr ni);
+          mret [instr]
+      | Unreachable => mret [wasm.BI_unreachable]
+      | Nop => mret [wasm.BI_nop]
+      (* | Drop => _ *)
+      (* | Select => _ *)
+      (* | Block tf le e__s => _ *)
+      (* | Loop tf e => _ *)
+      (* | ITE tf le e__thn e__els => _ *)
+      (* | Br i => _ *)
+      (* | Br_if i => _ *)
+      (* | Br_table i__s j => _ *)
+      (* | Ret => _ *)
+      (* | GetLocal i => _ *)
+      (* | SetLocal i => _ *)
+      (* | TeeLocal i => _ *)
+      (* | GetGlobal i => _ *)
+      (* | SetGlobal i => _ *)
+      (* | CallIndirect tf => _ *)
+      (* | Call i => _ *)
+      (* | LoadOffset offset => _ *)
+      (* | StoreOffset offset => _ *)
+      (* | SwapOffset offset => _ *)
+      (* | Malloc shape => _ *)
+      (* | Free => _ *)
+      | VariantCase q ψ tf le e__ss => mthrow (err "TODO: is this needed?")
+      | _ => mthrow (err "TODO")
+      end.
+
+
+
+
+
+  End Instrs.
+
+
+  Definition compile_function_types (tf : ArrowShape) (function_types : list wasm.function_type)
+    : list wasm.function_type :=
+
+   let function_type := translate_function_type tf in
+   add_if_not_in function_type function_types.
+
+  (* NOTE: could probably turn acculuation of function types into a monad but likely not worth it. *)
+  Definition compile_function (function : Func) (function_types : list wasm.function_type)
+    : M (list wasm.module_func * wasm.function_type).
+  Admitted.
+
+  Definition layout_compile_module (module : module) : M wasm.module :=
+    let 'Build_module functions globals table := module in
+    '(functions, function_types) ← foldlM ;
+
+    mret {|
+        wasm.mod_types := [];
+        wasm.mod_funcs := [];
+        wasm.mod_tables := []; (* TODO *)
+        wasm.mod_mems := []; (* TODO *)
+        wasm.mod_globals := []; (* TODO *)
+        wasm.mod_elem := []; (* TODO *)
+        wasm.mod_data := []; (* TODO *)
+        wasm.mod_start := None; (* TODO *)
+        wasm.mod_imports := []; (* TODO *)
+        wasm.mod_exports := [] (* TODO *)
+    |}.
+
+End LayoutToWasm.
